change field specs to use F

src/Bedrock/Specs/Field.v
@@ -1,13 +1,15 @@
 Require Import Rupicola.Lib.Api.
+Require Import Crypto.Algebra.Hierarchy.
+Require Import Crypto.Arithmetic.PrimeFieldTheorems.
 Local Open Scope Z_scope.
 
 Class FieldParameters :=
   { (** mathematical parameters **)
     M_pos : positive; (* modulus *)
     M : Z := Z.pos M_pos;
-    a24 : Z; (* (a+2) / 4 or (a-2) / 4, depending on the implementation *)
-    Finv : Z -> Z; (* modular inverse in Z/M *)
-    (** function names for bedrock2 **)
+    a24 : F M_pos; (* (a+2) / 4 or (a-2) / 4, depending on the implementation *)
+
+    (** function names **)
     mul : string; add : string; sub : string;
     square : string; scmula24 : string; inv : string;
 
@@ -27,9 +29,16 @@ Class FieldParameters :=
 Lemma M_nonzero {fp : FieldParameters} : M <> 0.
 Proof. cbv [M]. congruence. Qed.
 
-Class FieldRepresentation {semantics : Semantics.parameters} :=
+Class FieldParameters_ok {field_parameters : FieldParameters} :=
+  { M_prime : Znumtheory.prime M;
+    (* TODO: a24_ok *)
+  }.
+
+Class FieldRepresentation
+      {field_parameters : FieldParameters}
+      {semantics : Semantics.parameters} :=
   { felem : Type;
-    feval : felem -> Z;
+    feval : felem -> F M_pos;
     FElem : word -> felem -> Semantics.mem -> Prop;
     bounds : Type;
     bounded_by : bounds -> felem -> Prop;
@@ -54,7 +63,7 @@ Section Specs.
           ===> name @ [px; pout] ===>
           (fun _ =>
            liftexists out,
-           (emp ((feval out mod M = (op (feval x)) mod M)%Z
+           (emp (feval out = op (feval x)
                  /\ bounded_by outbounds out)
             * FElem pout out)%sep))
       (only parsing).
@@ -69,34 +78,23 @@ Section Specs.
           ===> name @ [px; py; pout] ===>
           (fun _ =>
            liftexists out,
-           (emp ((feval out mod M = (op (feval x) (feval y)) mod M)%Z
+           (emp ((feval out = op (feval x) (feval y))
                  /\ bounded_by outbounds out)
             * FElem pout out)%sep)) (only parsing).
 
-  Definition spec_of_mul : spec_of mul :=
-    binop_spec mul Z.mul loose_bounds loose_bounds tight_bounds.
-  Definition spec_of_square : spec_of square :=
-    unop_spec square (fun x => Z.mul x x) loose_bounds tight_bounds.
-  Definition spec_of_add : spec_of add :=
-    binop_spec add Z.add tight_bounds tight_bounds loose_bounds.
-  Definition spec_of_sub : spec_of sub :=
-    binop_spec sub Z.sub tight_bounds tight_bounds loose_bounds.
-  Definition spec_of_scmula24 : spec_of scmula24 :=
-    unop_spec scmula24 (Z.mul a24) loose_bounds tight_bounds.
-
+  Instance spec_of_mul : spec_of mul :=
+    binop_spec mul F.mul loose_bounds loose_bounds tight_bounds.
+  Instance spec_of_square : spec_of square :=
+    unop_spec square (fun x => F.mul x x) loose_bounds tight_bounds.
+  Instance spec_of_add : spec_of add :=
+    binop_spec add F.add tight_bounds tight_bounds loose_bounds.
+  Instance spec_of_sub : spec_of sub :=
+    binop_spec sub F.sub tight_bounds tight_bounds loose_bounds.
+  Instance spec_of_scmula24 : spec_of scmula24 :=
+    unop_spec scmula24 (F.mul a24) loose_bounds tight_bounds.
   (* TODO: what are the bounds for inv? *)
-  Definition spec_of_inv : spec_of inv :=
-    (forall! (x : felem) (px pout : word) (old_out : felem),
-        (fun Rr mem =>
-           bounded_by tight_bounds x
-           /\ (exists Ra, (FElem px x * Ra)%sep mem)
-           /\ (FElem pout old_out * Rr)%sep mem)
-          ===> inv @ [px; pout] ===>
-          (fun _ =>
-           liftexists out,
-           (emp ((feval out mod M = (Finv (feval x mod M)) mod M)%Z
-                 /\ bounded_by loose_bounds out)
-            * FElem pout out)%sep)).
+  Instance spec_of_inv : spec_of inv :=
+    unop_spec inv F.inv tight_bounds loose_bounds.
 
   Definition spec_of_felem_copy : spec_of felem_copy :=
     forall! (x : felem) (px pout : word) (old_out : felem),
@@ -110,7 +108,7 @@ Section Specs.
         ===> felem_small_literal @ [x; pout] ===>
         (fun _ =>
            liftexists X,
-           (emp (feval X mod M = word.unsigned x mod M
+           (emp (F.to_Z (feval X) = word.unsigned x
                  /\ bounded_by tight_bounds X)
             * FElem pout X)%sep).
 End Specs.
